libcrux-iot/sha3/proofs/lean/LibcruxIotSha3/Extraction/Funs.lean
@@ -4688,7 +4688,7 @@ def digest_size (mode : Algorithm) : RustM Std.Usize := do
   | Algorithm.Sha512 => ok SHA3_512_DIGEST_SIZE
 
 /-- [libcrux_iot_sha3::keccakx1]:
-    Source: 'sha3/src/lib.rs', lines 595:0-597:1 -/
+    Source: 'sha3/src/lib.rs', lines 620:0-622:1 -/
 def keccakx1
   (RATE : Std.Usize) (DELIM : Std.U8) (data : Slice Std.U8)
   (out : Slice Std.U8) :
@@ -4697,7 +4697,7 @@ def keccakx1
   keccak.keccak RATE DELIM data out
 
 /-- [libcrux_iot_sha3::sha512_ema]:
-    Source: 'sha3/src/lib.rs', lines 318:0-325:1
+    Source: 'sha3/src/lib.rs', lines 333:0-340:1
     Visibility: public -/
 def sha512_ema
   (digest : Slice Std.U8) (payload : Slice Std.U8) : RustM (Slice Std.U8) := do
@@ -4709,7 +4709,7 @@ def sha512_ema
   keccakx1 72#usize 6#u8 payload digest
 
 /-- [libcrux_iot_sha3::sha384_ema]:
-    Source: 'sha3/src/lib.rs', lines 281:0-288:1
+    Source: 'sha3/src/lib.rs', lines 291:0-298:1
     Visibility: public -/
 def sha384_ema
   (digest : Slice Std.U8) (payload : Slice Std.U8) : RustM (Slice Std.U8) := do
@@ -4721,7 +4721,7 @@ def sha384_ema
   keccakx1 104#usize 6#u8 payload digest
 
 /-- [libcrux_iot_sha3::sha256_ema]:
-    Source: 'sha3/src/lib.rs', lines 244:0-251:1
+    Source: 'sha3/src/lib.rs', lines 249:0-256:1
     Visibility: public -/
 def sha256_ema
   (digest : Slice Std.U8) (payload : Slice Std.U8) : RustM (Slice Std.U8) := do
@@ -4733,7 +4733,7 @@ def sha256_ema
   keccakx1 136#usize 6#u8 payload digest
 
 /-- [libcrux_iot_sha3::sha224_ema]:
-    Source: 'sha3/src/lib.rs', lines 207:0-214:1
+    Source: 'sha3/src/lib.rs', lines 212:0-219:1
     Visibility: public -/
 def sha224_ema
   (digest : Slice Std.U8) (payload : Slice Std.U8) : RustM (Slice Std.U8) := do
@@ -4805,7 +4805,7 @@ def sha224 (payload : Slice Std.U8) : RustM (Array Std.U8 28#usize) := do
   ok (index_mut_back s1)
 
 /-- [libcrux_iot_sha3::sha256]:
-    Source: 'sha3/src/lib.rs', lines 221:0-232:1
+    Source: 'sha3/src/lib.rs', lines 226:0-237:1
     Visibility: public -/
 def sha256 (payload : Slice Std.U8) : RustM (Array Std.U8 32#usize) := do
   let a := Array.repeat 32#usize 0#u8
@@ -4819,7 +4819,7 @@ def sha256 (payload : Slice Std.U8) : RustM (Array Std.U8 32#usize) := do
   ok (index_mut_back s1)
 
 /-- [libcrux_iot_sha3::sha384]:
-    Source: 'sha3/src/lib.rs', lines 258:0-269:1
+    Source: 'sha3/src/lib.rs', lines 263:0-274:1
     Visibility: public -/
 def sha384 (payload : Slice Std.U8) : RustM (Array Std.U8 48#usize) := do
   let a := Array.repeat 48#usize 0#u8
@@ -4833,7 +4833,7 @@ def sha384 (payload : Slice Std.U8) : RustM (Array Std.U8 48#usize) := do
   ok (index_mut_back s1)
 
 /-- [libcrux_iot_sha3::sha512]:
-    Source: 'sha3/src/lib.rs', lines 295:0-306:1
+    Source: 'sha3/src/lib.rs', lines 305:0-316:1
     Visibility: public -/
 def sha512 (payload : Slice Std.U8) : RustM (Array Std.U8 64#usize) := do
   let a := Array.repeat 64#usize 0#u8
@@ -4847,7 +4847,7 @@ def sha512 (payload : Slice Std.U8) : RustM (Array Std.U8 64#usize) := do
   ok (index_mut_back s1)
 
 /-- [libcrux_iot_sha3::shake128]:
-    Source: 'sha3/src/lib.rs', lines 332:0-343:1
+    Source: 'sha3/src/lib.rs', lines 352:0-363:1
     Visibility: public -/
 def shake128
   (BYTES : Std.Usize) (data : Slice Std.U8) : RustM (Array Std.U8 BYTES) := do
@@ -4862,14 +4862,14 @@ def shake128
   ok (index_mut_back s1)
 
 /-- [libcrux_iot_sha3::shake128_ema]:
-    Source: 'sha3/src/lib.rs', lines 352:0-354:1
+    Source: 'sha3/src/lib.rs', lines 372:0-374:1
     Visibility: public -/
 def shake128_ema
   (out : Slice Std.U8) (data : Slice Std.U8) : RustM (Slice Std.U8) := do
   keccakx1 168#usize 31#u8 data out
 
 /-- [libcrux_iot_sha3::shake256]:
-    Source: 'sha3/src/lib.rs', lines 361:0-372:1
+    Source: 'sha3/src/lib.rs', lines 386:0-397:1
     Visibility: public -/
 def shake256
   (BYTES : Std.Usize) (data : Slice Std.U8) : RustM (Array Std.U8 BYTES) := do
@@ -4884,28 +4884,28 @@ def shake256
   ok (index_mut_back s1)
 
 /-- [libcrux_iot_sha3::shake256_ema]:
-    Source: 'sha3/src/lib.rs', lines 381:0-383:1
+    Source: 'sha3/src/lib.rs', lines 406:0-408:1
     Visibility: public -/
 def shake256_ema
   (out : Slice Std.U8) (data : Slice Std.U8) : RustM (Slice Std.U8) := do
   keccakx1 136#usize 31#u8 data out
 
 /-- Trait implementation: [libcrux_iot_sha3::incremental::private::{impl libcrux_iot_sha3::incremental::private::Sealed for libcrux_iot_sha3::incremental::Shake128Xof}]
-    Source: 'sha3/src/lib.rs', lines 408:8-408:45 -/
+    Source: 'sha3/src/lib.rs', lines 433:8-433:45 -/
 @[reducible]
 def incremental.Shake128Xof.Insts.Libcrux_iot_sha3IncrementalPrivateSealed :
   incremental.private.Sealed incremental.Shake128Xof := {
 }
 
 /-- Trait implementation: [libcrux_iot_sha3::incremental::private::{impl libcrux_iot_sha3::incremental::private::Sealed for libcrux_iot_sha3::incremental::Shake256Xof}]
-    Source: 'sha3/src/lib.rs', lines 409:8-409:45 -/
+    Source: 'sha3/src/lib.rs', lines 434:8-434:45 -/
 @[reducible]
 def incremental.Shake256Xof.Insts.Libcrux_iot_sha3IncrementalPrivateSealed :
   incremental.private.Sealed incremental.Shake256Xof := {
 }
 
 /-- [libcrux_iot_sha3::incremental::{impl libcrux_iot_sha3::incremental::Xof<168usize> for libcrux_iot_sha3::incremental::Shake128Xof}::squeeze]:
-    Source: 'sha3/src/lib.rs', lines 489:8-491:9
+    Source: 'sha3/src/lib.rs', lines 514:8-516:9
     Visibility: public -/
 def incremental.Shake128Xof.Insts.Libcrux_iot_sha3IncrementalXof168.squeeze
   (self : incremental.Shake128Xof) (out : Slice Std.U8) :
@@ -4915,7 +4915,7 @@ def incremental.Shake128Xof.Insts.Libcrux_iot_sha3IncrementalXof168.squeeze
   ok ({ state := kxs }, out1)
 
 /-- [libcrux_iot_sha3::incremental::{impl libcrux_iot_sha3::incremental::Xof<168usize> for libcrux_iot_sha3::incremental::Shake128Xof}::absorb_final]:
-    Source: 'sha3/src/lib.rs', lines 485:8-487:9
+    Source: 'sha3/src/lib.rs', lines 510:8-512:9
     Visibility: public -/
 def
   incremental.Shake128Xof.Insts.Libcrux_iot_sha3IncrementalXof168.absorb_final
@@ -4926,7 +4926,7 @@ def
   ok { state := kxs }
 
 /-- [libcrux_iot_sha3::incremental::{impl libcrux_iot_sha3::incremental::Xof<168usize> for libcrux_iot_sha3::incremental::Shake128Xof}::absorb]:
-    Source: 'sha3/src/lib.rs', lines 477:8-479:9
+    Source: 'sha3/src/lib.rs', lines 502:8-504:9
     Visibility: public -/
 def incremental.Shake128Xof.Insts.Libcrux_iot_sha3IncrementalXof168.absorb
   (self : incremental.Shake128Xof) (input : Slice Std.U8) :
@@ -4936,7 +4936,7 @@ def incremental.Shake128Xof.Insts.Libcrux_iot_sha3IncrementalXof168.absorb
   ok { state := kxs }
 
 /-- [libcrux_iot_sha3::incremental::{impl libcrux_iot_sha3::incremental::Xof<168usize> for libcrux_iot_sha3::incremental::Shake128Xof}::new]:
-    Source: 'sha3/src/lib.rs', lines 468:8-472:9
+    Source: 'sha3/src/lib.rs', lines 493:8-497:9
     Visibility: public -/
 def incremental.Shake128Xof.Insts.Libcrux_iot_sha3IncrementalXof168.new
   : RustM incremental.Shake128Xof := do
@@ -4944,7 +4944,7 @@ def incremental.Shake128Xof.Insts.Libcrux_iot_sha3IncrementalXof168.new
   ok { state := kxs }
 
 /-- Trait implementation: [libcrux_iot_sha3::incremental::{impl libcrux_iot_sha3::incremental::Xof<168usize> for libcrux_iot_sha3::incremental::Shake128Xof}]
-    Source: 'sha3/src/lib.rs', lines 467:4-492:5 -/
+    Source: 'sha3/src/lib.rs', lines 492:4-517:5 -/
 @[reducible]
 def incremental.Shake128Xof.Insts.Libcrux_iot_sha3IncrementalXof168 :
   incremental.Xof incremental.Shake128Xof 168#usize := {
@@ -4960,7 +4960,7 @@ def incremental.Shake128Xof.Insts.Libcrux_iot_sha3IncrementalXof168 :
 }
 
 /-- [libcrux_iot_sha3::incremental::{impl libcrux_iot_sha3::incremental::Xof<136usize> for libcrux_iot_sha3::incremental::Shake256Xof}::squeeze]:
-    Source: 'sha3/src/lib.rs', lines 519:8-521:9
+    Source: 'sha3/src/lib.rs', lines 544:8-546:9
     Visibility: public -/
 def incremental.Shake256Xof.Insts.Libcrux_iot_sha3IncrementalXof136.squeeze
   (self : incremental.Shake256Xof) (out : Slice Std.U8) :
@@ -4970,7 +4970,7 @@ def incremental.Shake256Xof.Insts.Libcrux_iot_sha3IncrementalXof136.squeeze
   ok ({ state := kxs }, out1)
 
 /-- [libcrux_iot_sha3::incremental::{impl libcrux_iot_sha3::incremental::Xof<136usize> for libcrux_iot_sha3::incremental::Shake256Xof}::absorb_final]:
-    Source: 'sha3/src/lib.rs', lines 514:8-516:9
+    Source: 'sha3/src/lib.rs', lines 539:8-541:9
     Visibility: public -/
 def
   incremental.Shake256Xof.Insts.Libcrux_iot_sha3IncrementalXof136.absorb_final
@@ -4981,7 +4981,7 @@ def
   ok { state := kxs }
 
 /-- [libcrux_iot_sha3::incremental::{impl libcrux_iot_sha3::incremental::Xof<136usize> for libcrux_iot_sha3::incremental::Shake256Xof}::absorb]:
-    Source: 'sha3/src/lib.rs', lines 506:8-508:9
+    Source: 'sha3/src/lib.rs', lines 531:8-533:9
     Visibility: public -/
 def incremental.Shake256Xof.Insts.Libcrux_iot_sha3IncrementalXof136.absorb
   (self : incremental.Shake256Xof) (input : Slice Std.U8) :
@@ -4991,7 +4991,7 @@ def incremental.Shake256Xof.Insts.Libcrux_iot_sha3IncrementalXof136.absorb
   ok { state := kxs }
 
 /-- [libcrux_iot_sha3::incremental::{impl libcrux_iot_sha3::incremental::Xof<136usize> for libcrux_iot_sha3::incremental::Shake256Xof}::new]:
-    Source: 'sha3/src/lib.rs', lines 496:8-500:9
+    Source: 'sha3/src/lib.rs', lines 521:8-525:9
     Visibility: public -/
 def incremental.Shake256Xof.Insts.Libcrux_iot_sha3IncrementalXof136.new
   : RustM incremental.Shake256Xof := do
@@ -4999,7 +4999,7 @@ def incremental.Shake256Xof.Insts.Libcrux_iot_sha3IncrementalXof136.new
   ok { state := kxs }
 
 /-- Trait implementation: [libcrux_iot_sha3::incremental::{impl libcrux_iot_sha3::incremental::Xof<136usize> for libcrux_iot_sha3::incremental::Shake256Xof}]
-    Source: 'sha3/src/lib.rs', lines 495:4-522:5 -/
+    Source: 'sha3/src/lib.rs', lines 520:4-547:5 -/
 @[reducible]
 def incremental.Shake256Xof.Insts.Libcrux_iot_sha3IncrementalXof136 :
   incremental.Xof incremental.Shake256Xof 136#usize := {
